LambdaS5/tests/es5/eval_strict_var.in.js
@@ -1,0 +1,1 @@
+eval('"use strict"; var x = 1'); typeof(x)
