LambdaS5/coq/LjsExtraction.v
@@ -218,9 +218,6 @@ Set Extraction AccessOpaque.
 
 
 
-(* TODO exception handling to get None *)
-Extract Constant LjsCommon.desugar_expr => "fun s -> Some (Desugar.desugar (Batteries.String.of_list s))".
-
 Extract Constant Utils.string_of_nat => "fun n -> Batteries.String.to_list (string_of_int n)".
 
 Extract Constant LjsCommon.eq_number_decidable => "(=)".
